```
se ( C + D - B > 7 ou A + B >= C + D) então
    x recebe o valor de D * 2 + B *3
senão
    x recebe o valor de C + B * C + 5
fim se
escreva (x)
```

Considerando 
- A=2;
- B=5; 
- C=4; 
- D=3;

Substituindo os valores:
```
se ( 4 + 4 - 5 > 7 ou 2 + 5 >= 4 + 3) então
    x recebe o valor de 3 * 2 + 5 *3
senão
    x recebe o valor de 4 + 5 * 4 + 5
fim se
escreva (x)
```

Substituindo os valores:
```
se ( 3 > 7 ou 7 >= 7) então
    x recebe o valor de 3 * 2 + 5 *3
senão
    x recebe o valor de 4 + 5 * 4 + 5
fim se
escreva (x)
```

```
x recebe o valor de 3 * 2 + 5 *3
x recebe o valor de 6 + 15
x recebe o valor de 21
```

